Zero out policy register before running policy
This allows fixing the proof of sv_thm again (up to almost the same
level it was before, at least). There is one missing assumption still,
about the policy register being big enough for the sv policy (maybe that
assumption isn't required? since if not, you'll get back the default
policy anyway).

botworldScript.sml
@@ -176,10 +176,14 @@ val private_def = Define`
 val preamble_env_def = Define`
   preamble_env (ffi:'ffi ffi_state) = ARB:('ffi semanticPrimitives$state # v environment)`;
 
+val ffi_from_observation_def = Define`
+  ffi_from_observation obs m =
+    initial_ffi_state botworld_oracle
+      (encode_observation obs::clear_register 0 m)`;
+
 val run_policy_def = Define`
   run_policy obs k m =
-    let ffi = initial_ffi_state botworld_oracle
-      ((encode_observation obs)::m) in
+    let ffi = ffi_from_observation obs m in
     let (st,env) = preamble_env ffi in
     let policy = read_policy m in
     let (st',_) = evaluate_prog (st with clock := k) env policy in
